coq/simple/model.v
@@ -3,6 +3,9 @@
 Require Import Coq.Logic.FunctionalExtensionality.
 Require Import Coq.Classes.RelationClasses.
 Require Coq.Relations.Relation_Definitions.
+Require Import Coq.Classes.Equivalence.
+Require Import Coq.Classes.EquivDec.
+
 Require Import Lia.
 
 Require Export lc.tactics.
@@ -10,7 +13,9 @@ Require Export lc.scoped.
 Require Import structures.Structures.
 Require Export structures.consistency.
 
-Require Export denot.list_properties.
+Require Import structures.NFSet.
+
+Require Export denot.nelist_properties.
 
 Import MonadNotation.
 Open Scope monad_scope.
@@ -19,19 +24,128 @@ Local Open Scope set_scope.
 
 Import EnvNotations.
 
+Create HintDb examples.
+
 (* This is an  example of the graph model for the pure 
    untyped lambda calculus plus natural numbers. 
    
 *)
 
+(* 
 Lemma In_mem_fset {A}{v : A} : v ∈ mem (singleton_fset v).
 Proof. cbn. left. auto. Qed.
-#[export] Hint Resolve In_mem_fset : core.
+
 Lemma  valid_mem_singleton_fset {A}{v:A} :
   valid_mem (singleton_fset v).
 Proof. cbn. done. Qed.
-#[export] Hint Resolve valid_mem_singleton_fset : core.
+#[export] Hint Resolve valid_mem_singleton_fset : core. 
+*)
 (* ----------------------------------------------------------- *)
+
+
+(* NONEMPTY FINITE SETS *)
+(*
+Inductive nfset (A : Type) : Type := 
+  | NFSet : A -> list A -> nfset A.
+Arguments NFSet {_}.
+
+Definition singleton_nfset {A : Type} (x:A): nfset A := NFSet x nil.
+
+Definition union_nfset: forall {A : Type}, nfset A -> nfset A -> nfset A :=
+  fun {A} '(NFSet x xs) '(NFSet y ys) => NFSet x (y :: xs ++ ys).
+Definition In_nfset {A : Type}(x : A) '(NFSet y ys) : Prop :=
+  x = y \/ List.In x ys.
+Definition Included_nfset: forall {A : Type}, nfset A -> nfset A -> Prop :=
+  fun {A} (s1 s2: nfset A) => forall (x:A), In_nfset x s1 -> In_nfset x s2.
+Definition Equal_nfset {A:Type}(s1 s2 : nfset A) := 
+  Included_nfset s1 s2 /\ Included_nfset s2 s1.
+Definition Forall_nfset: forall {A : Type}, (A -> Prop) -> nfset A -> Prop := 
+  fun {A} Pr '(NFSet x xs) => Pr x /\ List.Forall Pr xs.
+Definition ForallT_nfset: forall {A : Type}, (A -> Type) -> nfset A -> Type :=
+  fun {A} Pr '(NFSet x xs) => (Pr x * List.ForallT Pr xs)%type.
+Definition mem : forall {A : Type}, nfset A -> P A := 
+  fun {A} (xs : nfset A) (x : A) => In_nfset x xs.
+
+#[export] Instance Symmetric_Equal_nfset: forall {A : Type}, nfset A -> Symmetric (@Equal_nfset A). Admitted.
+#[export] Instance Reflexive_Equal_nfset: forall {A : Type}, nfset A -> Reflexive (@Equal_nfset A). Admitted.
+#[export] Instance Transitive_Included_nfset: forall {A : Type}, nfset A -> Transitive (@Included_nfset A). Admitted.
+#[export] Instance Reflexive_Included_nfset: forall {A : Type}, nfset A -> Reflexive (@Included_nfset A). Admitted.
+#[export] Instance Transitive_Equal_nfset: forall {A : Type}, nfset A -> Transitive (@Equal_nfset A). Admitted.
+
+Lemma mem_In: forall {A : Type} {E : nfset A} (x : A), x ∈ mem E -> In_nfset x E. Admitted.
+Lemma mem_union: forall {A : Type} {E1 E2 : nfset A}, mem (union_nfset E1 E2) = (mem E1 ∪ mem E2). Admitted.
+Lemma mem_union_Included: forall {A : Type} {D1 D2 : nfset A} {w : P A},
+  mem D1 ⊆ w -> mem D2 ⊆ w -> mem (union_nfset D1 D2) ⊆ w. Admitted.
+Lemma mem_singleton {A}{v : A} : v ∈ mem (singleton_nfset v). Admitted.
+
+Lemma In_mem : forall {A : Type} {E : nfset A} (x : A), In_nfset x E -> x ∈ mem E. Admitted.
+Lemma mem_Forall: forall {A : Type} {E : nfset A} {Pr : A -> Prop}, Sets.Forall Pr (mem E) -> Forall_nfset Pr E.  Admitted.
+
+
+Lemma Forall_mem: forall {A : Type} {E : nfset A} {Pr : A -> Prop}, Forall_nfset Pr E -> Sets.Forall Pr (mem E). Admitted.
+Lemma Forall_sub_mem: forall {A : Type} {E : nfset A} (X : P A) (Pr : A -> Prop), mem E ⊆ X -> Sets.Forall Pr X -> Forall_nfset Pr E. Admitted.
+
+Lemma valid_mem_singleton: forall {A : Type}, nfset A -> forall x : A, valid (mem (singleton_nfset x)). Admitted.
+Lemma nonemptyT_mem: forall {A : Type} {E : nfset A}, nonemptyT (mem E). Admitted.
+Lemma valid_mem: forall {A : Type} {V : nfset A}, valid (mem V). Admitted.
+
+
+#[export] Hint Resolve 
+  Reflexive_Equal_nfset Reflexive_Included_nfset
+  mem_In mem_union mem_union_Included mem_singleton Forall_mem Forall_sub_mem 
+  In_mem
+  valid_mem_singleton nonemptyT_mem valid_mem : core.
+*)
+(*
+Definition eq_fset {A} : (fset A) -> fset A -> Prop := 
+  fun '(FSet xs) '(FSet ys) => forall x, (List.In x xs -> List.In x ys) /\ 
+                            forall x, (List.In x ys -> List.In x xs).
+
+Instance Eqfset {A} `{EqDec_eq A} : Equivalence (@eq_fset A).
+Admitted.
+
+
+Definition add_list {A}`{EqDec_eq A} (x : A) (xs : list A)  : list A := 
+  match In_dec_list x xs with 
+  | left _ => xs
+  | right _ => cons x xs
+  end.
+Definition add_fset {A}`{EqDec_eq A} (x : A) (f : fset A)  : fset A := 
+  let '(FSet xs) := f in FSet (add_list x xs) .
+
+Definition union_fset {A} `{EqDec_eq A}  (f : fset A) (g : fset A)  : fset A := 
+  let '(FSet xs) := f in 
+  fold_right add_fset g xs.                      
+
+  
+Lemma In_dec_list {A}`{EqDec_eq A} : 
+  forall (x : A) (xs : list A), { List.In x xs } + { not (List.In x xs) }.
+Proof.
+  intros x. induction xs. right. done.
+  destruct (H x a); subst.
+  - left. left. auto.
+  - destruct IHxs; subst.
+     + left. right. auto.
+     + right. intro h. inversion h. subst. done. done.
+Defined.
+
+
+*) 
+  
+(*
+Declare Scope nfset_scope.
+Open Scope nfset_scope.
+
+Module NFSetNotations.
+Notation " [ x ] " := (NFSet x nil) : nfset_scope.
+Notation " [ x ; y1 ; .. ; yn ] " := (NFSet x (cons y1 .. (cons yn nil) .. )) : nfset_scope.
+End NFSetNotations.
+*)
+
+Open Scope nfset_scope.
+Import NFSetNotations.
+
+(* ------------------------------------------------------------------------------------- *)
 
 
 (* The denotation of a lambda calculus function is as its "graph" or set of
@@ -39,33 +153,864 @@ Proof. cbn. done. Qed.
    
    Each pair in the set (i.e. v_map VS W) declares that if this value is
    applied to any value in VS, the result is W.
+
+   NOTE: because we don't have a unique representation for finite sets, 
+   we don't have a uniq representation for Values.
+
+   Solutions: work up to an equivalence of Values? yuck!
+   define "canonical" values based on a strict ordering? maybe
    
  *)
 
 (* begin Value *)
 Inductive Value : Type :=
   | v_nat : nat -> Value
-  | v_map : fset Value -> Value -> Value
+  | v_map : nfset Value -> Value -> Value
   | v_fun : Value.
 (* end Value *)
 
 #[export] Hint Constructors Value : core.
 
 
+Infix "↦" := v_map (right associativity, at level 80).
+Notation "∘" := v_fun.
+
+(* Here are some example values *)
+
+Definition f1  : Value  := [ ∘ ] ↦ ∘ .
+Definition f1' : Value  := [ f1 ] ↦ ∘.
+Definition f2  : Value  := [ ∘ ; f1 ] ↦ ∘.
+Definition f2' : Value  := [ f1' ] ↦ ∘. 
+Definition f3  : Value  := [ ∘ ; f1 ; f2 ] ↦ ∘.
+
+Definition g1  : Value  := [ ∘ ] ↦ f1 .
+Definition g1' : Value  := [ ∘ ] ↦ f1'.
+Definition g2  : Value  := [ ∘ ] ↦ f2.
+Definition g2' : Value  := [ ∘ ] ↦ f2'.
+Definition g3  : Value  := [ ∘ ] ↦ f3.
+
+(* 
+" \f. f 0 + f 1 " 
+   "{0 |-> 0, 1 -> 1} |-> 1"
+*)
+
+
+Fixpoint Value_ind' (P : Value -> Prop)
+       (n : forall n : nat, P (v_nat n))  
+       (m : forall (l : nfset Value) (w : Value), 
+           Forall_nfset P l -> P w -> P (v_map l w))
+       (f : P v_fun)
+       (v : Value) : P v := 
+  let rec :=  Value_ind' P n m f 
+  in
+  let fix rec_list (vs : list Value) : List.Forall P vs :=
+    match vs with 
+    | nil => List.Forall_nil _
+    | cons w ws => @List.Forall_cons Value P w ws (rec w) (rec_list ws)
+    end
+  in 
+  let rec_nfset (f : nfset Value) : Forall_nfset P f :=
+    match f with 
+    | NFSet v vs => conj (rec v) (rec_list vs)
+    end
+  in 
+  match v with 
+  | v_nat k => n k
+  | v_map X w => m X w (rec_nfset X) (rec w)
+  | v_fun => f
+  end.
+
+Fixpoint Value_rec' (P : Value -> Type)
+       (n : forall n : nat, P (v_nat n))  
+       (m : forall (l : nfset Value) (w : Value), 
+           ForallT_nfset P l -> P w -> P (v_map l w))
+       (f : P v_fun)
+       (v : Value) : P v := 
+  let rec :=  Value_rec' P n m f 
+  in
+  let fix rec_list (vs : list Value) : List.ForallT P vs :=
+    match vs with 
+    | nil => List.ForallT_nil _
+    | cons w ws => @List.ForallT_cons Value P w ws (rec w) (rec_list ws)
+    end
+  in 
+  let rec_nfset (f : nfset Value) : ForallT_nfset P f :=
+    match f with 
+    | NFSet v vs => (rec v , rec_list vs)
+    end
+  in 
+  match v with 
+  | v_nat k => n k
+  | v_map X w => m X w (rec_nfset X) (rec w)
+  | v_fun => f
+  end.
+
+
+Fixpoint Value_lt (v1 : Value) (v2 : Value) : Prop := 
+  let fix list_Value_lt (X : list Value) (Y : list Value) : Prop := 
+    match X , Y with 
+    | _   , nil => False
+    | nil , _   => True 
+    | cons x xs, cons y ys => Value_lt x y \/ (x = y /\ list_Value_lt xs ys)
+    end in
+  let fix nfset_lt (X : nfset Value) (Y : nfset Value) : Prop :=
+    match X , Y with 
+    | NFSet v1 vs1, NFSet v2 vs2 => 
+        Value_lt v1 v2 \/ (v1 = v2 /\ list_Value_lt vs1 vs2)
+    end in
+  match v1 , v2 with 
+  | v_nat k1 , v_nat k2 => Nat.lt k1 k2
+  | _ , v_nat _ => False
+  | v_nat _ , _ => True
+  | _ , v_fun => False
+  | v_fun  , _ => True
+  | v_map V1 w1 , v_map V2 w2 => 
+      nfset_lt V1 V2 \/ (V1 = V2 /\ Value_lt w1 w2)
+  end.
+
+Example lt1 : Value_lt ∘ f1. simpl; auto. Qed.
+Example lt2 : Value_lt f1 f2. simpl; auto. Qed.
+Example lt3 : Value_lt f2 f3. simpl; auto. tauto. Qed.
+ 
+#[export] Instance Irreflexive_Value_lt : Irreflexive Value_lt. Admitted.
+#[export] Instance Transitive_Value_lt : Transitive Value_lt. Admitted.
+
+(*
+Lemma eq_dec_list {A} : forall (l : list A), 
+ (List.ForallT (fun x : A => forall y : A, {x = y} + {x <> y}) l) -> 
+ forall f, { l = f } + { l <> f }.
+Proof.
+  intros l IH.
+  induction IH; intro f; destruct f.
+  - left; auto.
+  - right; done.
+  - right; done.
+  - destruct (p a); subst.
+    destruct (IHIH f); subst.
+    left; auto.
+    right. intro h. inversion h. done.
+    right. intro h. inversion h. done.
+Defined.
+*)
+
+Lemma eq_dec_Value : forall (x y : Value), { x = y } + { x <> y }.
+Proof.
+  intro x.
+  eapply Value_rec' with (v := x).
+  1: move=> n.
+  2: move=> l w IHl IHw.
+  all: move=> y; destruct y.
+  all: try solve [right; intro h; done].
+  all: try solve [left; auto].
+  - move: (eq_nat_dec n n0) => h. destruct h; subst. left; auto. 
+    right. intro h. inversion h. done.
+  - destruct (IHw y); subst.
+    destruct l as [l].
+    simpl in IHl.
+Admitted.
+
+#[export] Instance EqDec_eq_Value : EqDec_eq Value := eq_dec_Value.
+
+
+
+(* -------------------------------------------------------------- *)
+
+
+(* But there is a complication. We want to define application as follows:
+
+      APPLY D1 D2 = { w | (V ↦ w) in D1 /\ V ⊆ D2 }
+
+   In other words, the set of all results such that there is some mapping in
+   the function that matches the argument.
+
+   However, there is some redundancy in this definition.  If D1 is a set of
+   Values, such as
+   
+       { ∘, f1 , f1', f2 , f2', f3 }
+
+  then no matter what D2 we use, we will get the the *same* result from
+  application as if we had instead used the singleton set D1'
+
+       { f3 }
+
+   Why? because all applications that we can do with elements of this set, we
+   can do with f3.
+
+   This means that D1 and D1' are "observationally equal". So we would like
+   our definition of equality on sets to equate these two sets.
+
+   [ We also need to think about how approximation works with the codomain
+     type. ]
+
+   To capture this idea, we define an approximation between values (⊑) that
+   says when one value is superceded by another. (See below.) This relation is
+   a partial order: reflexive, transitive and (for canonical values)
+   antisymmetric.
+
+   For example, we have
+
+         ∘ ⊑ f1 ⊑ f2
+
+   We can extend this approximation to an ordering on sets with
+
+      D1 ⊑ D2 when forall x ∈ D1, exists y in D2 such that x ⊑ y
+
+   Our definition of equality for sets of values is the usual one:
+
+      D1 ≃ D2 when D1 ⊆ D2 and D2 ⊆ D1
+
+   It it is important that we can reason about equality of sets just by
+   reasoning about their contents. In other words, we have this extensional
+   reasoning principle:
+
+      forall X, D1 X <-> D2 X implies that D1 ≃ D2
+   
+   So we can't change our definition of set equality. But that means
+   application needs to produce equal sets with approximately equal arguments.
+
+   In other words, a property that we want is:
+
+      D1' ⊑ D1 -> APPLY D1' D2 ⊆ APPLY D1 D2
+
+  *)
+
+Definition approx_set approx (D1 : P Value) (D2 : P Value) : Prop :=
+  forall x, x ∈ D1 -> exists y, (y ∈ D2) /\ approx x y.
+
+Inductive approx : Value -> Value -> Prop := 
+  | a_nat : forall i, approx (v_nat i) (v_nat i)
+  | a_fun2 : approx v_fun v_fun
+  | a_fun1 : forall V w, 
+      approx v_fun (v_map V w)
+  | a_map : forall (V1 V2 : nfset Value) w1 w2,
+      approx_set approx (mem V1) (mem V2) ->
+      approx w1 w2 ->
+      approx (v_map V1 w1) (v_map V2 w2).
+
+#[export] Hint Constructors approx : core.
+
+Declare Scope Value_scope.
+Infix "⊑V" := approx (at level 80) : Value_scope.
+Open Scope Value_scope.
+
+Infix "⊑" := (approx_set approx) (at level 80).
+
+
+Ltac invert := 
+  repeat match goal with 
+  | [ H : _ ∈ mem (NFSet _ _) |- _ ] => inversion H; try done; subst; clear H 
+  | [ H : approx _ v_fun |- _ ] => inversion H; subst; clear H
+  | [ H : approx _ (_ _) |- _ ] => inversion H; subst; clear H
+  | [ H : In _ (_ :: _) |- _ ] => destruct H as [<- | ?]; subst; try done
+(*  | [ H : ?D1 ⊑ ?D2 , x : Value, xIn : x ∈ ?D1 |- _ ] => 
+      destruct (H x xIn) as [ y [ yIn h ]] *)
+  end.
+
+
+(* Some properties. *)
+
+Lemma Reflexive_approx {v} : approx v v.
+(*
+eapply Value_ind' with (P := fun x => approx x x); intros; eauto.
+econstructor; eauto.
+destruct l as [l].  simpl in H.
+rewrite Forall_forall in H. destruct H as [h1 h2].
+intros v1 v1In.
+inversion H1. subst. clear H1.
+destruct H5 as [h3 h4].
+rewrite Forall_forall in h4.
+destruct v1In; subst; try done.
+exists l. split; eauto. left. eauto.
+exists v1. split; eauto. right. auto.
+inversion H1. subst. clear H1.
+eauto.
+Qed.  *) Admitted.
+
+Instance Transitive_approx : Transitive approx.
+Admitted.
+
+#[export] Hint Resolve Reflexive_approx : core.
+
+Lemma Reflexive_approx_set {D} : D ⊑ D.
+Proof. intros x xIn. exists x. split; eauto. Qed.
+
+#[export] Hint Resolve Reflexive_approx_set : core.
+
+(* This is not true: our notion of approximation for nfsets is 
+   extensional. So we need to restrict this to canonical 
+   values below. *)
+Lemma antisymmetry_approx : forall x y, approx x y -> approx y x -> x = y.
+Proof.
+  intro x.
+  eapply Value_ind' with (P := fun x => forall y, approx x y -> approx y x -> x = y); eauto.
+  1: intro k.
+  2: intros V w IHV IHw.
+  all: intros y Axy Ayx.
+  all: inversion Ayx; try done; subst; clear Ayx.
+  all: inversion Axy; subst; clear Axy.
+  f_equal.
+  destruct V as [v1 VS1].
+  destruct V1 as [v2 VS2].
+  move: IHV => [IHv IHVS].
+Abort.
+
+
+(* ----- approx examples ------ *)
+  
+
+Lemma example_approx_nfset : forall V, mem V ⊑ mem [∘] -> (mem V ≃ mem [∘]).
+Proof. intros V A. destruct V as [y l]. 
+       split; intros z zIn.
+       - destruct zIn; subst.
+         move: (A y ltac:(left;eauto)) => [w [wIn h]].
+         inversion wIn; subst. inversion h. eauto. done.
+         move: (A z ltac:(right; eauto)) => [w [wIn h]].
+         inversion wIn; subst. inversion h. eauto. done.
+       - inversion zIn; subst; try done.
+         left.
+         move: (A y ltac:(left; eauto)) => [w [wIn h]].
+         inversion wIn; subst; try done. inversion h. auto.
+Qed.
+
+Lemma ordered_mem_circ : forall V1,
+  mem V1 ≃ mem [∘] ->
+  Forall_nfset (fun x => x = ∘) V1.
+Proof.
+  intros V1 EQ.
+  destruct V1.
+  move: v EQ.
+  induction l.
+  + intros v [h1 h2]. econstructor; eauto.
+    specialize (h1 v ltac:(left; eauto)). inversion h1. auto. done.
+  + intros v [h1 h2].  econstructor; eauto.
+    specialize (h1 v ltac:(left; eauto)). inversion h1. auto. done.
+    econstructor; eauto.
+    specialize (h1 a ltac:(right; left; eauto)). inversion h1. auto. done.
+    have h:  mem (NFSet v l) ≃ mem [∘].
+    { clear IHl. split.
+      intros z zIN. destruct zIN; subst. eapply h1. left; eauto.
+      eapply h1. right; right; eauto.
+      intros z zIn. destruct zIn; try done. subst.
+      move: (h2 ∘ ltac:(left; eauto)) => h3.
+      destruct h3 as [E1 | E2].  subst; left; eauto.
+      destruct E2; subst.
+      move: (h1 v ltac:(left; eauto)) => h4. destruct h4; try done. subst.
+      left; eauto.
+      right; eauto.
+    }
+    specialize (IHl v h). simpl in IHl. move: IHl => [h3 h4]. auto.
+Qed.
+
+
+
+
+(* Some examples of approx *)
+
+Example approx1 : approx ∘ f1 . cbv. eauto. Qed.
+
+Example approx2 : approx f1 f2. cbv. 
+econstructor; eauto with examples. 
+move=> v1 v1In. cbv in v1In. destruct v1In; try done. subst.
+exists ∘. split; cbn; eauto. Qed.
+
+Example approx1' : approx f1 f1'. cbv. econstructor; eauto with examples. 
+intros v1 v1In. cbv in v1In. destruct v1In; try done. subst.
+eexists. split. cbn. left; eauto. econstructor; eauto with examples. Qed.
+
+Example approx2' : approx f1' f2. cbv. econstructor; eauto with examples.
+move=> v1 v1In. cbv in v1In. destruct v1In; try done. subst.
+exists f1. split; cbv; eauto with examples. Qed.
+
+#[local]Hint Resolve approx1 approx2 approx1' approx2' : examples.
+
+
+
+(* --------------- maximal / complete --------------- *)
+
+(* The other issue that we need to address is that there are several 
+   representations for the same value. *)
+
+(* From this point on, we will work with *canonical* values only. *)
+
+(* A maximal set does not contain any strict approximations *)
+Definition maximal (D : P Value) :=
+  forall x y, x ∈ D -> y ∈ D -> (approx x y) -> x = y.
+
+Example maximal_singleton v : maximal (mem [v]).
+Proof. intros x y xIn yIn A. invert. Qed.
+
+#[export] Hint Resolve maximal_singleton : core.
+
+
+(* --------------- canonical values --------------- *)
+
+(* A canonical value is one where the nfset is 
+   strictly ordered
+
+   A complete canonical value is one where the nfset 
+   is also complete. We have to build this up in two steps 
+   because we want to be complete only over canonical 
+   values, not all values.
+ *)
+
+Inductive restricted (Pr : nfset Value -> Prop) : Value -> Prop := 
+  | restricted_v_nat : forall k, restricted Pr (v_nat k)
+  | restricted_v_fun : restricted Pr v_fun
+  | restricted_v_map : 
+    forall X w v VS, 
+      X = NFSet v VS ->
+      Pr X -> 
+      Forall_nfset (restricted Pr) (NFSet v VS) -> 
+      restricted Pr w -> 
+      restricted Pr (v_map X w).
+
+
+#[export] Hint Constructors restricted : core.
+
+Lemma restricted_impl : forall (P1 P2 : nfset Value -> Prop), 
+  (forall x, P1 x -> P2 x) -> forall v, restricted P1 v -> restricted P2 v.
+Proof. 
+  intros P1 P2 IM v.
+  eapply Value_ind' with (P := fun v => restricted P1 v -> restricted P2 v).
+  1: move=> i.
+  2: move=> l w IHl IHw.
+  all: move=> h; inversion h; subst; clear h.
+  all: eauto.
+  econstructor; eauto.
+  eapply mem_Forall.
+  rewrite Sets.Forall_forall.
+  intros x xIn.
+  apply Forall_mem in IHl.
+  apply Forall_mem in H3.
+  rewrite Sets.Forall_forall in IHl.
+  rewrite Sets.Forall_forall in H3.
+  eauto.
+Qed.
+
+(*
+Fixpoint ordered_list (v : Value) (xs: list Value) : Prop := 
+  match xs with 
+  | nil => True
+  | cons w ys => Value_lt v w /\ ordered_list w ys
+  end.
+
+Definition ordered_nfset '(NFSet v vs) := ordered_list v vs.
+
+(* This is the main property that we want from ordered nfsets *)
+Lemma ordered_extensional VS WS : 
+  ordered_nfset VS -> ordered_nfset WS -> mem VS ≃ mem WS -> VS = WS.
+Proof.
+Admitted.
+*)
+
+#[export] Instance StrictOrder_Value : StrictOrder Value_lt.
+Admitted.
+
+(* A canonical value orders all of the elements in v_map *)
+Definition canonical : Value -> Prop := restricted (ordered_nfset Value_lt).
+
+Definition canonical_nfset := Forall_nfset canonical.
+
+Definition canonical_set D := forall x, x ∈ D -> canonical x.
+
+Lemma mem_canonical {X} : canonical_nfset X -> canonical_set (mem X).
+Proof. destruct X as [v VS]. intros [h1 h2] x xIn.
+       destruct xIn as [->|h3]; auto. rewrite Forall_forall in h2. eauto. Qed.
+
+
+(* A complete set means that 
+   everything that approximates an element in V is already in V. *)
+Definition complete_nfset (V : nfset Value) := 
+  Forall_nfset (fun y => forall x, canonical x -> approx x y -> In_nfset x V) V.
+
+(* A complete set contains all of its approximations *)
+Definition complete_set (D : P Value) := forall D', Sets.Forall canonical D' -> D' ⊑ D -> D' ⊆ D.
+
+Lemma mem_complete {X} : complete_nfset X -> complete_set (mem X).
+Proof.
+  unfold complete_nfset, complete_set.
+  intros CX D' CD' APPROX. 
+  move: (Forall_mem CX) => CMX.
+  rewrite Sets.Forall_forall in CMX.
+  rewrite Sets.Forall_forall in CD'.
+  intros x xIn.
+  specialize (CD' x xIn).
+  move: (APPROX x xIn) => [y [yIn h]].
+  specialize (CMX y yIn x CD' h).
+  eapply In_mem. auto.
+Qed.
+
+
+(* complete/canonical values and sets *)
+Definition cc : Value -> Prop := 
+  restricted (fun X => ordered_nfset Value_lt X /\ complete_nfset X).
+
+Definition cc_nfset (V : nfset Value) := Forall_nfset cc V /\ complete_nfset V.
+
+Definition cc_set (D : P Value) := 
+  Sets.Forall cc D /\ forall D', Sets.Forall cc D' -> D' ⊑ D -> D' ⊆ D.
+
+Lemma mem_cc {X} : cc_nfset X -> cc_set (mem X).
+Proof.
+  unfold cc_nfset, cc_set, complete_nfset.
+  move=> [CCX CX].
+  split.
+  eauto.
+  intros D' ccD' APPROX.
+  intros x xIn.
+  eapply mem_complete; eauto.
+  rewrite Sets.Forall_forall.
+  rewrite Sets.Forall_forall in ccD'.
+  intros y yIn.
+  move: (ccD' y yIn) => h. unfold cc in h. unfold canonical.
+  eapply restricted_impl. 2: eapply h.
+  intros z [h1 h2]. done.
+Qed. 
+
+(* Two complete sets that approximate eachother are equal. *)
+Definition cc_approx_equality D1 D2 : 
+  cc_set D1 -> cc_set D2 
+  -> D1 ⊑ D2 -> D2 ⊑ D1 -> D1 ≃ D2.
+Proof.  unfold cc_set. intros [h1 h2][h3 h4] h5 h6. split; eauto. 
+Qed.
+
+
+(* Closure operation to force cc (sets). *)
+Definition close (D : P Value) : P Value :=
+  fun x => cc x /\ exists y, (y ∈ D) /\ approx x y.
+
+
+(* closed sets are cc *)
+Lemma cc_close D : cc_set (close D).      
+Proof.
+  split.
+  - unfold close. 
+    rewrite -> Sets.Forall_forall.
+    intros x xIn. destruct xIn. auto.
+  - intros D' CAN APP.
+    intros x xIn.
+    move: (APP x xIn) => [w [wIn h]].
+    move: wIn => [cw [y [yIn h3]]].
+    split. 
+    rewrite -> Sets.Forall_forall in CAN. eauto.
+    exists y. split; eauto. transitivity w; auto.
+Qed.
+
+Lemma close_mono : forall D1 D2, D1 ⊆ D2 -> close D1 ⊆ close D2.
+Proof.
+  intros D1 D2 SUB.
+  intros x [h1 [y [yIn h2]]].
+  split; auto. exists y.  split. eapply SUB; eauto. auto.
+Qed.  
+
+
+(* Two cc elements that approximate eachother are equal. *)
+
+Lemma approx_antisymmetry x:
+  forall y, cc x -> cc y -> 
+       approx x y -> approx y x -> x = y.
+Proof.
+  eapply Value_ind' with (P := fun x =>   forall y, cc x -> cc y -> approx x y -> approx y x -> x = y).
+  1: intros n.
+  2: intros V w IHV IHw.
+  all: intros y Cx Cy Axy Ayx.
+  all: inversion Ayx; subst; clear Ayx.
+  all: auto.
+  - inversion Axy.
+  - inversion Axy. subst. clear Axy.
+    inversion Cx. subst. clear Cx.
+    inversion Cy. subst. clear Cy.
+    f_equal. 2: eauto.
+    match goal with 
+    | [ H7 : ordered_nfset Value_lt (NFSet v VS) /\ complete_nfset _ |- _ ] => move: H7 => [OX CX] end.
+    match goal with 
+    | [ H7 : ordered_nfset Value_lt (NFSet v0 VS0) /\ complete_nfset _ |- _ ] => move: H7 => [OX0 CX0] end.
+
+    eapply ordered_extensional; eauto using StrictOrder_Value. 
+    eapply cc_approx_equality; eauto.
+    eapply mem_cc. split; eauto.
+    eapply mem_cc. split; eauto.
+Qed.    
+
+(*                        
+    
+Definition maximal_approx_subset D1 D2 : 
+  canonical_set D1 -> canonical_set D2 ->
+  maximal D1 ->
+  D1 ⊑ D2 -> D2 ⊑ D1 -> D1 ⊆ D2.
+Proof.  
+  intros C1 C2 M1 S1 S2. 
+  intros x xIn.
+  destruct (S1 x xIn) as [w [wIn hw]].
+  destruct (S2 w wIn) as [z [zIn hz]].
+  have AZ: approx x z. transitivity w; auto.
+  have EQ: x = z. eapply M1; eauto. subst z.
+  have EQ: w = x. eapply approx_antisymmetry; eauto.
+  subst. done.
+Qed.
+
+Definition maximal_approx_equality D1 D2 : 
+  canonical_set D1 -> canonical_set D2 ->
+  maximal D1 -> maximal D2 ->
+  D1 ⊑ D2 -> D2 ⊑ D1 -> D1 ≃ D2.
+Proof.  
+  intros C1 C2 M1 M2 S1 S2. 
+  split; eauto using maximal_approx_subset.
+Qed. *)
+
+
+(* CC Examples *)
+
+Example cc_f0 : cc ∘.
+Proof. repeat econstructor; eauto. Qed.
+#[local] Hint Resolve cc_f0 : examples.
+
+Example cc_nfset_f0 : cc_nfset [∘].
+Proof. repeat econstructor; eauto. invert. auto. Qed.
+#[local] Hint Resolve cc_nfset_f0 : examples.
+
+Example cc_f1 : cc f1.
+Proof. repeat econstructor; eauto. invert. auto. Qed.
+#[local] Hint Resolve cc_f1 : examples.
+
+Example cc_nfset_f1 : cc_nfset [∘; f1].
+Proof. econstructor; eauto.
+       econstructor; eauto with examples.
+       unfold complete_nfset.
+       econstructor.
+       - intros x Cx xA. invert. econstructor; eauto.
+       - econstructor; eauto.
+         intros x Cx Ax.
+         unfold f1 in Ax.
+         inversion Ax; subst; clear Ax.
+         + econstructor; eauto.
+         + inversion Cx; subst; clear Cx.
+           inversion H3; subst. clear H3.
+           remember (NFSet v VS) as X. 
+           have EQ: X = [∘].
+           { eapply ordered_extensional; eauto with examples. 
+             eapply StrictOrder_Value.
+             econstructor; eauto.
+             eapply example_approx_nfset; eauto. }
+           right. left. subst. rewrite EQ. unfold f1. done.
+Qed.                        
+#[local] Hint Resolve cc_nfset_f1 : examples.
+
+Example cc_f2 : cc f2.
+Proof.
+  move: cc_nfset_f1 => [h1 h2].
+  econstructor; eauto with examples.
+  split; eauto.
+  econstructor; simpl; eauto. 
+Qed.
+
+#[local] Hint Resolve cc_f2 : examples.
+
+
+(*
+
+(* Furthermore, values are finite, so we can *calculate* the (finite) set of values that 
+   approximate a specific value. 
+
+*)
+
+Definition fset_of_list {A}`{EqDec_eq A} (l : list A) : fset A := 
+  fold_right add_fset empty_fset l.
+
+Definition unFSet {A} : fset A -> list A := 
+  fun '(FSet xs) => xs.
+
+Definition flat_map_fset {A B}`{EqDec_eq A}`{EqDec_eq B} (f : A -> fset B) : fset A -> fset B := 
+  fun '(FSet xs)  => 
+    fset_of_list (flat_map (fun x => unFSet (f x)) xs).
+
+
+Fixpoint powerset {A}`{EqDec_eq A} (l : list A) : list (fset A) :=
+    match l with 
+    | nil => cons [] nil
+    | cons x xs =>
+        ps <- powerset xs ;;
+        cons (add_fset x ps) (powerset xs)
+    end.
+
+Lemma powerset_spec {A}{D :EqDec_eq A} (x : list A) :
+  forall (y : fset A), List.In y (powerset x) -> mem y ⊆ mem (FSet x).
+Proof.
+  induction x.
+  - intros. simpl in *. destruct H; try done. subst.
+    reflexivity.
+  - intros y tIn. simpl in *.
+    rewrite in_flat_map_Exists in tIn.
+    inversion tIn; subst; clear tIn.
+    + inversion H0; subst; clear H0.
+      ++ rewrite <- H in IHx.
+         specialize (IHx x0 ltac:(left; eauto)).
+         move=>z zIn. 
+         destruct x0 as [x0].
+         unfold add_fset, add_list in zIn.
+         destruct (In_dec_list a x0).
+         right. eapply IHx. cbn. auto.
+         destruct zIn. subst. left. auto.
+         cbn. right. eapply IHx. cbn. auto.
+      ++ rewrite <- H in IHx.
+         specialize (IHx y ltac:(eauto)).
+         move=>z zIn. cbn. right. eapply IHx. eauto.
+    + rewrite <- H in IHx.
+      rewrite Exists_nth in H0.
+      destruct H0 as [i [d [ID InY]]].
+      move: (nth_In l d ID) => h.
+      destruct InY.
+      ++ specialize (IHx (List.nth i l d) ltac:(right;eauto)).
+         rewrite <- H0.
+         intros z zIn.
+         remember (List.nth i l d) as Z.
+         destruct Z as [z0].
+         unfold add_fset, add_list in zIn.
+         destruct (In_dec_list a z0).
+         right. eapply IHx. done.
+         destruct zIn. subst. left. auto.
+         right. eapply IHx. 
+         move: H1. clear.  induction z0. intros. done.
+         intros h. destruct h. subst. left. auto. 
+         specialize (IHz0 H). right. eauto.
+      ++ specialize (IHx y H0). 
+         intros z zIn. right. eapply IHx. eauto.
+Qed.         
+
+Fixpoint approximates (v : Value) : list Value := 
+  match v with 
+  | v_nat k => cons (v_nat k) nil
+  | v_fun => cons v_fun nil
+  | v_map (FSet xs) w =>
+      add_list v_fun
+      (W1 <- (powerset (flat_map approximates xs)) ;;
+       w1 <- (approximates w) ;;
+       cons (W1 ↦ w1) nil)
+  end.
+
+
+Definition approximates_fset (W : fset Value) : list (fset Value) :=
+  let '(FSet xs) := W in powerset (flat_map approximates xs).
+
+Lemma aproximates_spec : forall v w, 
+    approx w v <->
+    List.In w (approximates v).
+Admitted.
+*)
+
+Lemma sub_union {A} {X Y Z W: P A}: X ⊆ Z -> Y ⊆ W -> (X ∪ Y) ⊆ (Z ∪ W).
+Proof. intros s1 s2.
+       intros x xIn.
+       destruct xIn.
+       left; eauto.
+       right; eauto.
+Qed.
+
+(* We need an operation that computes the closure of a single value. *)
+Definition close_nfset : Value -> nfset Value. Admitted.
+
+Lemma approx_union {D X Y} : D ⊑ (X ∪ Y) -> exists D1, exists D2, (D1 ⊑ X) /\ (D2 ⊑ Y) /\ (D ≃ (D1 ∪ D2)).
+Proof. intros. 
+       unfold approx_set in H.
+       exists (fun x => (x ∈ D) /\ exists y, (y ∈ X) /\ (approx x y)).
+       exists (fun x => (x ∈ D) /\ exists y, (y ∈ Y) /\ (approx x y)).
+       repeat split.
+       - intros x Pr.
+         destruct Pr as [xIn [y [yIn yA]]]. exists y; split; eauto.
+       - intros x Pr.
+         destruct Pr as [xIn [y [yIn yA]]]. exists y; split; eauto.
+       - intros x xIn.
+         cbv.
+         move: (H x xIn) => [y [yIn yA]].
+         destruct yIn.
+         left. split; eauto.
+         right. split;  eauto.
+       - intros x xIn.
+         destruct xIn.
+         move: H0 => [ xIn _]; auto.
+         move: H0 => [ xIn _]; auto.
+Qed.         
+
+Lemma cc_union X Y :  cc_set X  -> cc_set Y -> cc_set (X ∪ Y).
+  intros [X1 X2] [Y1 Y2].
+  repeat rewrite Sets.Forall_forall in X1 Y1.
+  split.
+  - (* union is canonical *)
+    rewrite Sets.Forall_forall.
+    intros x [xX | xY]; eauto.
+  - (* union is complete *)
+    intros D' ccD' DAPP.
+    rewrite Sets.Forall_forall in ccD'. 
+    move: (approx_union DAPP) => [D1 [D2 [D1A [D2A EQ]]]].
+    move: EQ => [h1 h2].
+    have canD1 : Sets.Forall cc D1.
+    { 
+      rewrite Sets.Forall_forall.
+      intros y yIn. apply ccD'. apply h2. left. auto.
+    }
+    have canD2 : Sets.Forall cc D2.
+    { 
+      rewrite Sets.Forall_forall.
+      intros y yIn. apply ccD'. apply h2. right. auto.
+    }
+    transitivity (D1 ∪ D2); auto.
+    eapply sub_union; eauto.
+Qed.
+    
+                      
+Instance Validity_Valid : Validity Value.
+apply MkValid with (validT_set := fun X => (nonemptyT X * cc_set X)%type).
+- intros X [NE CC].
+  destruct NE. 
+  have CCx: cc x. move: CC => [h1 h2]. rewrite Sets.Forall_forall in h1. auto.
+  (* need to show that we can close a single element and produce a finite set. *)
+  admit.  
+- intros X [NE CC]. auto.
+- intros X Y [NEX CCX] [NEY CCY].
+  split. 
+  + move: NEX => [x xIn]. exists x. left; auto.
+  + eapply cc_union; eauto.
+Admitted. 
+
+
 (* --- semantic operators -------  *)
+
+(*
+Definition maximize (D : P Value) : P Value := 
+  fun x => (x ∈ D) /\ forall y, y ∈ D -> approx x y -> x = y.
+
+Lemma maximal_maximize D : maximal (maximize D).
+Proof. intros x y xIn yIn A. move: xIn => [xIn mX].
+       move: yIn => [yIn mY]. eauto. Qed.
+*)
 
 Inductive LAMBDA (f : P Value -> P Value) : P Value :=
   | s_map : forall V w, 
+      cc (v_map V w) ->
       w ∈ f (mem V) ->
-      valid_mem V ->
       LAMBDA f (v_map V w)
-  | s_fun : LAMBDA f v_fun. 
+  | s_fun : 
+      LAMBDA f v_fun.
+
+(* Does application produce a maximal result??? *)
+
+(* 
+   Say D1 = { 1 ↦ ∘ } { 2 ↦ f0 }
+       D2 = { 1 , 2 }
+   then
+       APPLY D1 D2 = { ∘ , f0 }    
+   
+   which is not maximal
+
+*)
+  
 
 (* begin APPLY *)
 Inductive APPLY : P Value -> P Value -> (Value -> Prop) :=
-  | BETA : forall D1 D2 w V,
-     (v_map V w) ∈ D1 ->
-     (mem V ⊆ D2) -> valid_mem V ->
+  | BETA : forall D1 D2 V w,
+      (v_map V w ∈ D1) -> 
+      (mem V ⊆ D2) -> 
+      cc (v_map V w) ->
      APPLY D1 D2 w.
 (* end APPLY *)
 
@@ -73,11 +1018,13 @@ Inductive NAT (k : nat) : P Value :=
   | s_Nat : NAT k (v_nat k).
 
 Inductive ADD : P Value :=
-  | s_ADD : forall i j k V1 V2,
-      v_nat i ∈ mem V1 ->
-      v_nat j ∈ mem V2 -> 
+  | s_ADD : forall i j k,
       k = i + j ->
-      ADD (v_map V1 (v_map V2 (v_nat k))).
+      ADD (v_map [ v_nat i ] (v_map [v_nat j] (v_nat k))).
+(*  | s_ADD2 : forall i V1,
+      ⌈ v_nat i ⌉ ≃ mem V1 ->
+      ADD (v_map V1 v_fun)
+  | s_ADD3 : ADD v_fun. *)
 
 #[export] Hint Constructors Value LAMBDA APPLY NAT ADD : core.
 
@@ -87,33 +1034,339 @@ Ltac invert_sem :=
   | [ H : ?x ∈ APPLY ?v1 ?v2 |- _ ] => inversion H; subst; clear H
   | [ H : ?x ∈ NAT ?k |- _ ] => inversion H; subst; clear H
   | [ H : ?x ∈ ADD |- _ ] => inversion H; subst; clear H
+  | [ H : ?x ∈ close ?D |- _ ] => 
+      let h1 := fresh "cc" in 
+      let w  := fresh "w" in
+      let wIn := fresh "IN" in
+      let APP := fresh "APP" in
+      move: H => [ h1 [w [wIn APP]]] 
   end.
+
+
+(* --------------- canonical_set --------------------------------- *)
+
+Lemma cc_set_Bottom : cc_set Bottom.
+Proof. 
+unfold cc_set. split; eauto. 
+rewrite Sets.Forall_forall. intros x xIn. inversion xIn.
+intros D ccD APP x xIn. destruct (APP x xIn) as [w [wIn h]].  done.
+Qed.
+
+#[export] Hint Resolve cc_set_Bottom : examples.
+
+Lemma cc_set_NAT k : cc_set (NAT k).
+unfold cc_set. split; eauto. 
+rewrite Sets.Forall_forall. intros x xIn. inversion xIn.
+unfold cc. econstructor; eauto.
+intros D ccD APP x xIn. destruct (APP x xIn) as [w [wIn h]].  
+invert_sem. invert. econstructor; eauto.
+Qed.
+
+#[export] Hint Resolve cc_set_NAT : examples.
+
+
+(*
+Lemma canonical_set_APPLY D1 D2 : 
+  canonical_set D1 -> 
+  canonical_set (APPLY D1 D2).
+Proof. 
+  intros C1.
+  intros x xIn.
+  invert_sem.
+  inversion H1.
+  auto.
+Qed.
+
+Lemma canonical_set_LAMBDA : forall F, canonical_set (LAMBDA F).
+Proof.
+  intros.
+  intros x xIn.
+  invert_sem; eauto.
+Qed. *)
+
+
+
+(* --------------- maximal  --------------------------------- *)
+
+(*
+Definition canonical_dom X :=
+  ordered_nfset X /\
+  maximal (mem X) /\
+  Forall_nfset canonical X.
+
+
+Lemma coapprox : forall y x1 x2, 
+    canonical x1 -> canonical x2 -> canonical y ->
+    approx x1 y -> approx x2 y -> approx x1 x2 \/ approx x2 x1.
+Proof.
+  intro y.
+  eapply Value_ind' with (P := fun y => forall x1 x2, 
+                                   canonical x1 -> canonical x2 -> canonical y ->
+                                   approx x1 y -> approx x2 y -> approx x1 x2 \/ approx x2 x1).
+  1: move=>n.
+  2: move=>V w IHV IHw.
+  all: intros x1 x2 C1 C2 C A1 A2.
+  all: inversion C; subst; clear C.
+  all: inversion A1; inversion A2; subst; clear A1 A2.
+  all: try solve [left; eauto].
+  all: try solve [right; eauto].
+  inversion C1. inversion C2. subst. clear C1 C2.
+  destruct (IHw w1 w0); eauto.
+  - remember (NFSet v0 VS0) as X1.
+    remember (NFSet v1 VS1) as X2.
+    remember (NFSet v VS) as X.
+    left.
+Abort.
+
+Lemma maximal_approx : forall D, 
+    maximal D ->  
+    forall X1 X2, 
+      canonical_dom X1 -> canonical_dom X2 ->
+      mem X1 ⊑ D -> mem X2 ⊑ D -> 
+      exists X, (mem X ⊑ D) /\ (mem X1 ⊑ mem X) /\ (mem X2 ⊑ mem X).
+Proof. 
+  intros D mD X1 X2 C1 C2 A1 A2.
+Admitted. *)
+
+(*
+Lemma maximal_Bottom : maximal Bottom.
+Proof. 
+intros x y xIn yIn. inversion xIn.
+Qed.
+*)
+
+(*
+Lemma maximal_APPLY D1 D2 : 
+  maximal D1 ->
+  maximal D2 -> 
+  maximal (APPLY D1 D2).
+Proof. 
+  intros C1 C2.
+  intros x y xIn yIn A.
+  invert_sem.
+  invert_sem.
+  destruct H as [V1 [In1 [h1 CVw1]]].
+  destruct H1 as [V2 [In2 [h2 CVw2]]].
+(*   specialize (H0 V2 x In2 h2 CVw2). *)
+  specialize (H2 V1 y In1 h1 CVw1).
+  inversion CVw1. inversion CVw2. subst.
+  eapply approx_antisymmetry; eauto.
+Qed.
+
+Lemma maximal_LAMBDA : forall F, (forall X, maximal X -> maximal (F X)) -> maximal (LAMBDA F).
+Proof.
+  intros.
+  intros x y xIn yIn A.
+  invert_sem. invert_sem.
+  all: inversion A; subst; clear A.
+  - inversion H0. inversion H2. subst. clear H0. clear H2.
+    remember (NFSet v0 VS0) as X0.
+    remember (NFSet v VS) as X.
+    move: (H _ H10) => MF.
+    move: (H _ H17) => MF0.
+  -  specialize (H1 V w H). 
+  - auto.
+Qed.
+*)
+
+
+(*
+Lemma maximal_NAT i : maximal (NAT i).
+Proof.
+  intros x y xIn yIn APPROX.
+  repeat invert_sem. eauto.
+Qed.
+
+Lemma maximal_ADD : maximal ADD.
+Proof.
+  intros x y xIn yIn APP.
+  repeat invert_sem.
+  repeat invert.
+  move: (H2 (v_nat i0) ltac:(left;eauto)) => [v [vIn h2]].
+  move: (H3 (v_nat j0) ltac:(left;eauto)) => [w [wIn h3]].
+  destruct vIn; try done; subst.
+  destruct wIn; try done; subst.
+  invert.
+  auto.
+Qed. *)
+
+(* ------------------ complete ---------------------- *)
+
+(* If we have a complete set, it works as well as any of its approximations in an application. *)
+
+(*
+Lemma complete_sub : forall D1, maximal D1 -> forall D1', D1' ⊑ D1 -> forall D2, 
+        APPLY D1' D2 ⊆ APPLY D1 D2.
+Proof.
+  intros.
+  intros x xIn.
+  invert_sem.
+  eapply BETA; eauto. 
+  unfold maximal in H.
+  eapply H in H0; eauto.
+Qed.
+*)
+
+(*
+Lemma complete_Bottom : complete Bottom.
+Proof. intros x A y yIn. cbv in A.
+destruct (A y yIn) as [v [h _]]. done.
+Qed. *)
+
+(*
+Lemma complete_APPLY D1 D2 : 
+  complete D1 -> 
+  complete (APPLY D1 D2).
+Proof. intros C1.
+       intros x A y yIn.
+       destruct (A y yIn) as [z [zIn h]].
+       invert_sem.
+       have CVz: canonical (V ↦ y).
+       { inversion H1. subst. econstructor; eauto using approx_canonical_sub. }
+       econstructor; eauto.
+       eapply C1 with (D' := ⌈ V ↦ y ⌉); eauto.
+       intros w wIn. inversion wIn; subst. exists (V ↦ z). split; eauto.
+       econstructor; eauto.
+       eapply Reflexive_approx_set.
+       inversion H1. subst.
+       eapply mem_canonical. eauto.
+Qed.       
+
+Lemma complete_LAMBDA : forall F, (forall D, complete D -> complete (F D)) -> complete (LAMBDA F).
+Proof.
+  intros.
+  intros x A y yIn.
+  destruct (A y yIn) as [z [zIn h]].
+  invert_sem;  inversion h; subst; clear h.
+  - econstructor; eauto.
+  - move: (H _ H2) => CFD.
+    econstructor; eauto.
+    inversion H9.
+
+inversion yIn; subst; econstructor; auto. clear yIn.
+  inversion y. clear y. subst.  
+  inversion H6. subst.
+  move: (H (mem V) H2) => h.
+  unfold complete in h.
+  have C1: complete (mem V1).
+  { unfold complete. intros x xIn.
+    move: (H3 x xIn) => [v2 [h1 h2]].
+    move=> y cy A.
+    
+
+  move: (H (mem V1) H2) => h.
+
+Admitted. *)
+
+Lemma singleton_nat i V1 V0 : 
+  ⌈ v_nat i ⌉ ≃ mem V1 ->
+  mem V0 ⊑ mem V1 -> 
+  ⌈ v_nat i ⌉ ≃ mem V0.
+Proof.
+  intros.
+  destruct V0.
+  split.
+  - intros x xIn. inversion xIn. subst .
+    move: (H0 v ltac:(left; auto)) => [v1 [h1 h2]].
+    rewrite <- H in h1. inversion h1. subst. clear h1.
+    inversion h2. subst. clear h2.
+    left; auto.
+  - intros x xIn. 
+    move: (H0 x xIn) => [v1 [h1 h2]].
+    rewrite <- H in h1. inversion h1. subst. clear h1.
+    inversion h2. subst. clear h2.
+    eauto.
+Qed.
+
+(*
+Lemma complete_NAT i : complete (NAT i).
+  intros x xIn y cy yIn.
+  invert_sem; inversion yIn; subst; clear yIn; eauto.
+  econstructor; eauto.
+Qed.  
+
+Lemma complete_ADD : complete ADD.
+  intros x xIn y cy yIn.
+  invert_sem; inversion yIn; subst; clear yIn; eauto.
+  - econstructor. 
+  - inversion H5; subst; eauto; clear H5.
+    econstructor; eauto.
+    instantiate (1 := i).
+    eapply singleton_nat; eauto.
+    inversion H7; subst; clear H7.
+    econstructor; eauto.
+    eapply singleton_nat; eauto.
+    eapply singleton_nat; eauto.
+  - econstructor; eauto.
+  - inversion H4. subst. clear H4.
+    econstructor; eauto.
+    eapply singleton_nat; eauto.
+  - econstructor; eauto.
+Qed.
+
+
+#[export] Hint Resolve complete_Bottom : core.
+*)
+
 
 (* Denotation function *)
 
-Import LCNotations.
-
-Open Scope tm.
-
 Definition Rho := list (P Value).
+
 
 (* Denotation function *)
 Fixpoint denot (a : tm) (ρ : Rho) : P Value :=
      match a with 
      | var_b n => ρ ⋅ n 
 
-     | abs t => LAMBDA (fun D => denot t (D :: ρ))
+     | abs t => close (LAMBDA (fun D => denot t (D :: ρ)))
 
-     | app t u   =>  APPLY (denot t ρ) (denot u ρ)
+     | app t u   =>  close (APPLY (denot t ρ) (denot u ρ))
 
      | lit i => NAT i
 
-     | add   => ADD
+     | add   => close ADD
 
      | _ => Bottom
      end.
 
 (* --------------- monotonicity ------------------------------ *)
+
+(*
+(* MAXIMIZE is not monotonic. We may have to kick out some values.... *)
+Lemma maximize_mon_sub {D1 D2} : 
+  D1 ⊆ D2 -> maximize D1 ⊆ maximize D2.
+Proof.
+  intros SUB x xIn.
+  destruct xIn as [xIn h].
+  move: (SUB x xIn) => xIn2.
+  split. auto.
+  intros; eauto.
+Abort. *)
+
+Lemma approx_sub : forall D1 D2 D3, D1 ⊑ D2 -> D2 ⊆ D3 -> D1 ⊑ D3.
+Proof.
+  intros.
+  intros x xIn.
+  move: (H x xIn) => [y [yIn h]].
+  exists y. split; eauto.
+Qed.
+
+
+Lemma close_cong { D1 D3 } :
+    D1 ≃ D3 -> (close D1 ) ≃ (close D3 ).
+Proof.
+  intros [ d13 d31 ].
+  split; eapply close_mono; eauto.
+Qed.
+
+
+#[export] Instance Proper_Included_close : Proper (Included ==> Included) close. 
+unfold Proper. intros x1 y1 E1. eapply close_mono; eauto. Qed.
+
+#[export] Instance Proper_Same_close : Proper (Same_set ==> Same_set) close. 
+unfold Proper. intros x1 y1 E1. eapply close_cong; eauto. Qed.
+
 
 (* Λ-ext-⊆  *)
 
@@ -137,11 +1390,22 @@ Qed.
 Lemma APPLY_mono_sub { D1 D2 D3 D4 } :
     D1 ⊆ D3 -> D2 ⊆ D4 -> ((APPLY D1 D2) ⊆ (APPLY D3 D4)).
 Proof.  
-  intros D13 D24 w APP. 
+  intros D13 D24 w wIn. 
   invert_sem.
-  apply BETA with (V:=V); eauto.
-  intros d z. eauto.
+  eapply BETA with (V := V); eauto.
+(*   eapply approx_sub; eauto. *)
+  transitivity D2; auto.
 Qed.
+
+(*
+Lemma maximal_APPLY_mono_sub { D1 D2 D3 D4 } :
+    D1 ⊆ D3 -> D2 ⊆ D4 -> ((maximal_APPLY D1 D2) ⊆ (maximal_APPLY D3 D4)).
+Proof.  
+  intros D13 D24 w [APP mAPP]. 
+  split. eapply APPLY_mono_sub; eauto.
+  intros y yIn SUB.
+Abort. *)
+
 
 Lemma APPLY_cong { D1 D2 D3 D4 } :
     D1 ≃ D3 -> D2 ≃ D4 -> ((APPLY D1 D2) ≃ (APPLY D3 D4)).
@@ -170,10 +1434,13 @@ Proof.
   all: try move=> ρ1 ρ2 SUB.
   all: try reflexivity.
   - eapply access_mono_sub; eauto.
-  - eapply LAMBDA_ext_sub; eauto.
-    move=> X neX.
-    eapply IHt; eauto.
-  - eapply APPLY_mono_sub; eauto.
+  - simpl. simpl in H.
+    eapply close_mono with (D1 := LAMBDA (fun D => denot t (D :: t1))).
+    eapply LAMBDA_ext_sub; eauto.
+    auto.
+  - simpl.
+    eapply close_mono.
+    eapply APPLY_mono_sub; eauto.
 Qed.
 
 (* The denotation respects ≃ *)
@@ -210,18 +1477,114 @@ Qed.
 
 (* ------------------ valid ---------------------- *)
 
-Lemma valid_LAMBDA : forall F, valid (LAMBDA F).
-Proof. intros F. cbv. exists v_fun. auto. Qed.
+Lemma valid_close : forall D, valid D -> Sets.Forall cc D -> valid (close D).
+Proof. intros D vD ccD. destruct vD as [w wIn].
+exists w. split. eapply ccD; eauto. exists w. split; eauto.
+Qed.
+
+Lemma cc_set_LAMBDA : forall F, Sets.Forall cc (LAMBDA F).
+Proof. intros F. 
+rewrite Sets.Forall_forall. intros x xIn.
+inversion xIn; auto. eauto with examples.
+Qed.
+
+Lemma valid_LAMBDA : forall F, valid (close (LAMBDA F)).
+Proof. intros F. exists v_fun. split. eauto with examples.
+exists ∘. split. eapply s_fun. eauto. Qed.
 
 Lemma valid_NAT : forall k, valid (NAT k).
 Proof. intros k. cbv. exists (v_nat k). econstructor; eauto. Qed.
 
-Lemma valid_ADD : valid ADD.
-Proof. cbv. exists (v_map (singleton_fset (v_nat 0)) (v_map (singleton_fset (v_nat 0)) (v_nat 0))).
-       econstructor; cbv; eauto. 
+Lemma cc_v_nat k : cc (v_nat k).
+Proof. econstructor; eauto. Qed.
+
+Lemma cc_nfset_nat k : cc_nfset (singleton_nfset (v_nat k)).
+Proof.
+  unfold cc_nfset.
+  split.
+  econstructor; eauto. econstructor.
+  unfold complete_nfset.
+  econstructor; eauto.
+  intros x xC xA.
+  invert.
+  eauto.
+Qed.
+
+#[export] Hint Resolve cc_v_nat cc_nfset_nat : examples.
+
+Lemma valid_ADD : valid (close ADD).
+Proof. 
+  exists (v_map (singleton_nfset (v_nat 0)) 
+            (v_map (singleton_nfset (v_nat 0)) (v_nat 0))).
+  split.
+  - have hO: ordered_nfset Value_lt (singleton_nfset (v_nat 0)).  simpl; auto.
+    have hC: complete_nfset (singleton_nfset (v_nat 0)). 
+    { econstructor; eauto. intros x cX aX. invert. eauto. }
+    eapply restricted_v_map. reflexivity.
+    split; auto. 
+    econstructor; eauto.
+    eapply restricted_v_map. reflexivity.
+    split; auto.
+    econstructor; eauto.
+    eauto.
+  - exists (v_map (singleton_nfset (v_nat 0)) 
+            (v_map (singleton_nfset (v_nat 0)) (v_nat 0))).
+    split. econstructor; eauto. 
+    econstructor; eauto.
+Qed.
+
+Lemma Forall_access {A} : forall Pr ρ (d:A) k, List.Forall Pr ρ -> Pr d -> Pr (access d ρ k).
+Proof. Admitted.
+
+Lemma denot_complete : forall t ρ, List.Forall cc_set ρ -> cc_set (denot t ρ).
+Proof.
+  induction t.
+  all: simpl; intros ρ CR.
+  all: eauto with examples.
+  - eapply Forall_access; eauto with examples.
+  - eapply cc_close.
+  - eapply cc_close.
+  - eapply cc_close.
 Qed.
 
 (* ------------------ continuity ---------------------- *)
+
+(*
+Definition continuous {A} (F : P Value -> P A) : Set :=
+  forall X E, mem E ⊆ F X -> valid X -> cc_set X 
+         -> exists D, (cc_nfset D) /\ (mem D ⊆ X) /\ ((mem E) ⊆ F (mem D)).
+
+Definition continuous_In {A} (D:Rho Value -> P A) (ρ:Rho Value) (v:A) : Prop :=
+  v ∈ D ρ -> exists ρ' , exists (pf : finite_env ρ'),  ρ' ⊆e ρ /\ (v ∈ D ρ').
+
+Definition continuous_env {A} (D:Rho Value -> P A) (ρ:Rho Value) : Prop :=
+  forall (v : A), continuous_In D ρ v.
+
+Definition continuous_Sub {A} (D:Rho Value -> P A) (ρ:Rho Value) (V:nfset A) : Prop :=
+  mem V ⊆ D ρ -> 
+  exists ρ', exists (pf : finite_env ρ'),
+    ρ' ⊆e ρ  /\ (mem V ⊆ D ρ').
+*)
+
+
+(* ------------------ continuity ---------------------- *)
+
+Lemma close_continuous_env {D : Rho -> P Value}{ρ} :
+  (validT_env ρ)
+  -> continuous_env D ρ 
+  -> monotone_env (dom ρ) D 
+  -> continuous_env (fun ρ => close (D ρ)) ρ.
+Proof.  
+  intros NE IHD mD.
+  unfold continuous_env in IHD.
+  intros V h SUB VE.
+  destruct (IHD V ltac:(auto)) as 
+      [ ρ1 [ fρ1 [ ρ1ρ VwDp1 ]]]; auto.
+  exists ρ1. exists fρ1. split. auto.
+  split. auto.
+  exists y. split; auto.
+Qed. 
+
 
 Lemma APPLY_continuous_env {D E : Rho -> P Value}{ρ} :
   (nonempty_env ρ)
@@ -263,16 +1626,16 @@ Qed.
 *)
 
 Lemma LAMBDA_continuous_env {E ρ} {NE : nonempty_env ρ} :
-    (forall V, valid_mem V -> continuous_env E (mem V :: ρ))
+    (forall V, valid (mem V) -> continuous_env E (mem V :: ρ))
   -> monotone_env (S (dom ρ)) E
   -> continuous_env (fun ρ => LAMBDA (fun D => E (D :: ρ))) ρ.
 Proof.
   intros IH mE.
   intros v vIn.
-  inversion vIn as [ f w wEVρ VV EQ | ]. subst; clear vIn.
+  inversion vIn as [ V w CCfw wEVρ EQ | ]. subst; clear vIn.
   - (* v is V ↦ w *)
-    have NEx: nonempty_env (mem f :: ρ). econstructor; eauto.
-    specialize (IH f ltac:(eauto) w wEVρ).
+    have NEx: nonempty_env (mem V :: ρ). econstructor; eauto.
+    specialize (IH V ltac:(eauto) w wEVρ).
     destruct IH as [ρ' [F' [S' h']]].
     inversion S'. subst. inversion F'. subst.
     exists l. eexists. eauto.
@@ -285,22 +1648,6 @@ Proof.
     repeat split; eauto. 
     econstructor.
 Qed.
-
-(*
-Lemma access_continuous_env {A} : 
-forall (ρ : list (P A)) (x : nat),
-       nonempty_env ρ ->
-       continuous_env (fun ρ0  => access (fun _ : A => False) ρ0 x) ρ.
-Admitted.
-
-
-
-Lemma extend_valid_env {A} {ρ : list (P A)}{X} : 
-  valid X -> 
-  nonempty_env ρ -> nonempty_env (X :: ρ).
-Proof. intros NEP NEX.  eapply List.ForallT_cons; eauto. Qed.
-#[export] Hint Resolve extend_valid_env : core.
-*)
 
 (* ⟦⟧-continuous *)
 Lemma denot_continuous_env {t} : forall ρ,
@@ -316,16 +1663,23 @@ Proof.
   - (* var case *)
     eapply access_continuous_env; eauto.
   - (* abs *)
+    eapply close_continuous_env; eauto.
     eapply LAMBDA_continuous_env; eauto using denot_monotone.
+    intros ρ1 ρ2 DE SUB; 
+    eapply LAMBDA_ext_sub; intros X VX; eapply denot_monotone; eauto.
     Unshelve. eauto.
   - (* app *)
+    eapply close_continuous_env; eauto.
     eapply APPLY_continuous_env; eauto using denot_monotone.
+    intros ρ1 ρ2 DE SUB; eapply APPLY_mono_sub; eapply denot_monotone; eauto.
   - (* lit *)
     inversion cIn; subst;
     exists (initial_finite_env ρ NE); repeat split; eauto. 
   - (* add *)
+    eapply close_continuous_env; eauto.
     inversion cIn; subst;
     exists (initial_finite_env ρ NE); repeat split; eauto. 
+    intros ρ1 ρ2 DE SUB. reflexivity.
 Qed.
 
 (* --------------------------------------------------- *)
@@ -340,8 +1694,7 @@ Proof.
   intros NE_ρ V VinEρ.
   eapply generic_continuous_sub;
     eauto using denot_continuous_env, denot_monotone.
-Qed.
-
+Qed. 
 
 (* ⟦⟧-continuous-one *)
 Lemma denot_continuous_one { t ρ } :
@@ -356,29 +1709,66 @@ Proof.
   + eauto.
   + inversion h1. subst. inversion pf. subst.
     match goal with [H6 : finite x |- _ ] => move: H6 => [D [S NN]] end.
-    exists D. split.
-    rewrite <- S. auto.
-    split. 
+    exists D. split. transitivity x; auto.
     have SUB: List.Forall2 Included 
                 (x :: l) (mem D :: ρ).
     econstructor; eauto. 
-    rewrite <- S. reflexivity.
-    rewrite <- SUB. eapply h2. 
-    eapply valid_sub_valid_mem; eauto. rewrite <- S. auto. 
+    transitivity (denot t (x :: l)); auto.
+    eapply denot_monotone; eauto.
 Qed.
 
 (*  ----- Abstraction followed by Application is the identity -------- *)
 
+Lemma same_dom V V0 w0 w2 : 
+  cc (V ↦ w0) ->
+  cc (V0 ↦ w2) ->
+  mem V ⊑ mem V0 ->
+  mem V ⊆ mem V0.
+Proof.
+  intros c1 c2 APP. inversion c1; inversion c2; clear c2 c2.
+  subst X0. subst w1. subst X. subst w.
+  split_hyp.
+  
+  move: (mem_complete H0) => h0.
+  unfold complete_set in h0.
+  have CV: Sets.Forall canonical (mem V). admit.
+  specialize (h0 (mem V) CV APP).
+  auto.
+Admitted.
+
+Definition cc_fun F := forall X, cc_set X -> cc_set (F X).
+
+
+
 (* Λ-▪-id *)
 Lemma LAMBDA_APPLY_id { F X } :
-  continuous F -> monotone F -> valid X
-  -> APPLY (LAMBDA F) X ≃ F X.
+  continuous F -> monotone F -> cc_fun F -> valid X -> cc_set X 
+  -> close (APPLY (close (LAMBDA F)) X) ≃ F X.
 Proof. 
-  intros Fcont Fmono NEX.
+  intros Fcont Fmono Fcc NEX Xcc.
   split.
-  + intros w APP. inversion APP; subst.
-    - invert_sem. 
-      specialize (Fmono (mem V) X ltac:(auto)).
+  + intros w wIn. invert_sem. invert_sem. invert_sem. invert_sem; invert.
+    admit.
+  + intros w wInFX.
+    move: (Fcc X Xcc) => [ccFX compFX]. rewrite Sets.Forall_forall in ccFX.
+    move: (ccFX _ wInFX) => ccw.
+    split; auto.
+    exists w. split. 
+    have M : mem (singleton_nfset w) ⊆ F X. { intros d y. inversion y; subst. auto. done. }
+    move: (Fcont X (singleton_nfset w) M NEX) => [ D [ DltX wInFD ]].
+    have CCDw: cc (D ↦ w).
+    { destruct D as [v V]. eapply restricted_v_map. eauto.
+      split.
+    eapply BETA with (V := D); eauto.
+    split.
+
+    ++ have EQ: V = V0. {
+         inversion cc1. inversion H. subst.
+         destruct H7. destruct H14.
+      have II: mem (singleton_nfset w2) ⊆ F X. { intros w1 w1In. inversion w1In. subst.
+      move: (Fcont X (singleton_nfset w2)) => h. [ D [ DltX [ wInFD NED ]]].
+specialize (Fmono (mem V) X ltac:(auto)).
+Admitted. (*
       eauto.
   + intros w wInFX.
     have M: mem (singleton_fset w) ⊆ F X. 
@@ -387,7 +1777,7 @@ Proof.
     [ D [ DltX [ wInFD NED ]]].
     eapply BETA with (V:=D); eauto.
     eapply s_map; eauto.
-Qed.
+Qed. *)
 
 
 (* Λ⟦⟧-▪-id *)
@@ -395,7 +1785,7 @@ Lemma LAMBDA_denot_APPLY_id :
   forall t ρ X,
     valid X
     -> nonempty_env ρ
-    -> (APPLY (LAMBDA (fun D => denot t  (D :: ρ))) X) ≃
+    -> close (APPLY (close (LAMBDA (fun D => denot t  (D :: ρ)))) X) ≃
       denot t (X  ::  ρ).
 Proof.
   intros.
@@ -414,10 +1804,12 @@ Ltac invert_sub :=
   end.
   
 
-Lemma APPLY_ADD i j : APPLY (APPLY ADD (NAT i)) (NAT j) ≃ (NAT (i+j)).
+
+Lemma APPLY_ADD i j : close (APPLY (close (APPLY (close ADD) (NAT i))) (NAT j)) ≃ (NAT (i+j)).
 Proof.
 split.
 - intros x xIn.
+  unfold close in xIn.
   repeat invert_sem.
   repeat invert_sub.
   econstructor; eauto.
@@ -429,49 +1821,49 @@ split.
   eapply In_mem_Included. cbv; eauto.
   eapply In_mem_Included. cbv; eauto.
 Qed.
-
+*)
 
 (* ------------------- beta reduction is sound ----------------- *)
 
-(*
+Definition open (t : tm) (u : tm) : tm. Admitted.
+
 Lemma subst_denot1 :
   forall (t : tm) (u : tm) (ρ : list (P Value)),
-    scoped t (denot u ρ :: ρ) 
-    -> scoped u ρ 
-    -> valid (denot u ρ)
+(*    scoped t (denot u ρ :: ρ) 
+    -> scoped u ρ  *)
+      valid (denot u ρ)
     -> nonempty_env ρ
-    -> denot t (denot u ρ :: ρ) ≃ denot (t [x ~> u]) ρ.
+    -> denot t (denot u ρ :: ρ) ≃ denot (open t u) ρ.
 Proof.
-Admitted.
+Admitted. 
+
+
 
 
 Lemma beta_soundness : forall t u ρ, 
-  scoped (abs t) ρ ->
-  scoped u ρ -> 
+(*   scoped (abs t) ρ ->
+  scoped u ρ ->  *)
   nonempty_env ρ ->
   valid (denot u ρ) -> 
-  denot (app (abs t) u) ρ ≃ denot (open_tm_wrt_tm t u) ρ.
+  denot (app (abs t) u) ρ ≃ denot (open t u) ρ.
 Proof.
-  intros t u ρ St Su NE V.
-  pick fresh x.
-  rewrite denot_app.
-  rewrite (denot_abs x); auto.
+  intros t u ρ NE V.
+  simpl.
   rewrite (LAMBDA_denot_APPLY_id); auto.
   rewrite subst_denot1; eauto.
-  eapply scoped_abs_inv; eauto.
-  rewrite (subst_tm_intro x t u); auto.
   reflexivity.
 Qed.
-*)
 
 (* ------------------------ examples --------------------------- *)
 
-Lemma In_valid_mem {A} {x : A}{f}: x ∈ mem f -> valid_mem f.
+(*
+Lemma In_valid_mem {A} {x : A}{f}: x ∈ mem f -> valid (mem f).
 Proof. intro xIn.  destruct f.
        intro h. subst. done.
 Qed.
 
 #[export] Hint Resolve In_valid_mem : core.
+*)
 
 (* 3 + 4 is 7 *)
 
@@ -522,6 +1914,21 @@ Proof.
   + cbn in xIn.
     eapply s_map; eauto.
 Qed.
+
+
+(* \f.\x. f x *)
+Definition tm_eta_Id := abs (abs (app (var_b 1) (var_b 0))).
+
+Lemma denot_eta_Id : denot tm_eta_Id nil ⊆ idset.
+Proof.
+  simpl.
+  move=> x xIn.
+  invert_sem; try done.
+  invert_sem; try done.
+  invert_sem; try done.
+  cbn. admit. 
+  cbn. admit.
+Abort.
 
 (* Example: constant function K -- \x. \y. x n *)
 
