coq/denot/properties.v
@@ -5,6 +5,7 @@ Require Import Lia.
 
 Require Export lc.tactics.
 Require Import structures.Structures.
+Require Import structures.FSet.
 Require Export structures.consistency.
 
 
